checkpoint

TotalUtil.thy
@@ -35,14 +35,14 @@ lemma update_trace_total_heap_same: "get_hh_total_full (update_trace_total \<ome
 lemma update_trace_total_mask_same: "get_mh_total_full (update_trace_total \<omega> \<pi>) = get_mh_total_full \<omega>"
   by simp
 
-definition update_heap_total :: "'a total_state \<Rightarrow> heap_loc \<Rightarrow> 'a val \<Rightarrow> 'a total_state"
-  where "update_heap_total \<phi> l v = Abs_total_state ( ((get_mh_total \<phi>), (get_hh_total \<phi>)(l := v)), get_pmh_total \<phi>)"
+definition update_hh_loc_total :: "'a total_state \<Rightarrow> heap_loc \<Rightarrow> 'a val \<Rightarrow> 'a total_state"
+  where "update_hh_loc_total \<phi> l v = Abs_total_state (((get_hh_total \<phi>)(l := v), get_hp_total \<phi>), get_m_total \<phi>)"
 
-definition update_mask_total :: "'a total_state \<Rightarrow> mask \<Rightarrow> 'a total_state"
-  where "update_mask_total \<phi> m' = Abs_total_state ((m', get_hh_total \<phi>), get_pmh_total \<phi>)"
+definition update_mh_total :: "'a total_state \<Rightarrow> mask \<Rightarrow> 'a total_state"
+  where "update_mh_total \<phi> mh = Abs_total_state (get_h_total \<phi>, (mh, get_mp_total \<phi>))"
 
-definition update_pmask_total :: "'a total_state \<Rightarrow> 'a predicate_mask \<Rightarrow> 'a total_state"
-  where "update_pmask_total \<phi> pm = Abs_total_state (get_mh_total \<phi>, (pm, get_pheap_total \<phi>))"
+definition update_mp_total :: "'a total_state \<Rightarrow> 'a predicate_mask \<Rightarrow> 'a total_state"
+  where "update_mp_total \<phi> mp = Abs_total_state (get_h_total \<phi>, (get_mh_total \<phi>, mp))"
 
 lemma Abs_total_state_inverse_2:
   assumes "wf_pre_total_state (m,h)"
@@ -50,22 +50,22 @@ lemma Abs_total_state_inverse_2:
   using assms Abs_total_state_inverse
   by blast
 
-lemma get_update_mask_total: 
+lemma get_update_mh_total: 
   assumes "wf_mask_simple m0"
-  shows   "get_mh_total (update_mask_total mh m0) = m0"
-  unfolding update_mask_total_def
+  shows   "get_mh_total (update_mh_total mh m0) = m0"
+  unfolding update_mh_total_def
   using assms
   by (simp add: Abs_total_state_inverse_2)
 
-lemma update_mask_total_multiple: 
+lemma update_mh_total_multiple: 
   assumes "wf_mask_simple m0" and "wf_mask_simple m2"
-  shows   "update_mask_total (update_mask_total mh m0) m1 = update_mask_total mh m1"
-  unfolding update_mask_total_def  
+  shows   "update_mh_total (update_mh_total mh m0) m1 = update_mh_total mh m1"
+  unfolding update_mh_total_def  
   using assms
   by (simp add: Abs_total_state_inverse_2)
 
-lemma update_heap_total_mask_same: "get_mh_total (update_heap_total \<phi> l v) = get_mh_total \<phi>"
-  unfolding update_heap_total_def
+lemma update_hh_loc_total_mask_same: "get_mh_total (update_hh_loc_total \<phi> l v) = get_mh_total \<phi>"
+  unfolding update_hh_loc_total_def
   (*
   by (metis Abs_total_state_inverse_2 fst_conv get_mh_total.simps get_mh_total_wf wf_pre_total_state.simps)*)
   sorry
@@ -73,85 +73,89 @@ lemma update_heap_total_mask_same: "get_mh_total (update_heap_total \<phi> l v) 
 lemma Rep_total_state_inj: "Rep_total_state a = Rep_total_state b \<Longrightarrow> a = b"
   by (metis Rep_total_state_inverse)
 
-lemma update_heap_total_overwrite: "update_heap_total (update_heap_total mh l v1) l v2 = update_heap_total mh l v2"
+lemma update_hh_loc_total_overwrite: "update_hh_loc_total (update_hh_loc_total mh l v1) l v2 = update_hh_loc_total mh l v2"
  (* apply (rule total_state_eq)
-   apply (simp only: update_heap_total_mask_same)
-  by (metis Abs_total_state_inverse_2 fun_upd_upd get_hh_total.simps get_mh_total_wf snd_conv update_heap_total_def wf_pre_total_state.simps)*)
+   apply (simp only: update_hh_loc_total_mask_same)
+  by (metis Abs_total_state_inverse_2 fun_upd_upd get_hh_total.simps get_mh_total_wf snd_conv update_hh_loc_total_def wf_pre_total_state.simps)*)
   sorry
 
-lemma update_heap_total_lookup_1: "get_hh_total (update_heap_total \<phi> l v) l = v"
- (* by (metis (no_types, lifting) Abs_total_state_inverse_2 fun_upd_eqD fun_upd_triv get_hh_total.simps get_mh_total_wf snd_conv update_heap_total_def wf_pre_total_state.simps) *)
+lemma update_hh_loc_total_lookup_1: "get_hh_total (update_hh_loc_total \<phi> l v) l = v"
+ (* by (metis (no_types, lifting) Abs_total_state_inverse_2 fun_upd_eqD fun_upd_triv get_hh_total.simps get_mh_total_wf snd_conv update_hh_loc_total_def wf_pre_total_state.simps) *)
   sorry
 
-lemma update_heap_total_lookup_2: "l1 \<noteq> l2 \<Longrightarrow> get_hh_total (update_heap_total \<phi> l1 v) l2 = get_hh_total \<phi> l2"
-(*  by (metis (no_types, lifting) Abs_total_state_inverse_2 fun_upd_idem_iff fun_upd_triv fun_upd_twist get_hh_total.elims get_mh_total_wf sndI update_heap_total_def wf_pre_total_state.simps) *)
+lemma update_hh_loc_total_lookup_2: "l1 \<noteq> l2 \<Longrightarrow> get_hh_total (update_hh_loc_total \<phi> l1 v) l2 = get_hh_total \<phi> l2"
+(*  by (metis (no_types, lifting) Abs_total_state_inverse_2 fun_upd_idem_iff fun_upd_triv fun_upd_twist get_hh_total.elims get_mh_total_wf sndI update_hh_loc_total_def wf_pre_total_state.simps) *)
   sorry
 
-fun update_heap_total_full :: "'a full_total_state \<Rightarrow> heap_loc \<Rightarrow> 'a val \<Rightarrow> 'a full_total_state"
-  where "update_heap_total_full \<omega> l v = (get_store_total \<omega>, get_trace_total \<omega>, update_heap_total (get_total_full \<omega>) l v )"
+fun update_hh_loc_total_full :: "'a full_total_state \<Rightarrow> heap_loc \<Rightarrow> 'a val \<Rightarrow> 'a full_total_state"
+  where "update_hh_loc_total_full \<omega> l v = (get_store_total \<omega>, get_trace_total \<omega>, update_hh_loc_total (get_total_full \<omega>) l v )"
 
-lemma update_heap_total_full_lookup_1: "get_hh_total_full (update_heap_total_full \<phi> l v) l = v"
-  by (metis get_hh_total_full.simps get_total_full.simps snd_conv update_heap_total_full.simps update_heap_total_lookup_1)
+lemma update_hh_loc_total_full_lookup_1: "get_hh_total_full (update_hh_loc_total_full \<phi> l v) l = v"
+  by (metis get_hh_total_full.simps get_total_full.simps snd_conv update_hh_loc_total_full.simps update_hh_loc_total_lookup_1)
 
-lemma update_heap_total_full_lookup_2: "l1 \<noteq> l2 \<Longrightarrow> get_hh_total_full (update_heap_total_full \<phi> l1 v) l2 = get_hh_total_full \<phi> l2"
-  by (metis get_hh_total_full.simps get_total_full.simps snd_conv update_heap_total_full.simps update_heap_total_lookup_2)
+lemma update_hh_loc_total_full_lookup_2: "l1 \<noteq> l2 \<Longrightarrow> get_hh_total_full (update_hh_loc_total_full \<phi> l1 v) l2 = get_hh_total_full \<phi> l2"
+  by (metis get_hh_total_full.simps get_total_full.simps snd_conv update_hh_loc_total_full.simps update_hh_loc_total_lookup_2)
 
-lemma update_heap_total_overwrite_full: "update_heap_total_full (update_heap_total_full \<omega> l v1) l v2 = update_heap_total_full \<omega> l v2"
+lemma update_hh_loc_total_overwrite_full: "update_hh_loc_total_full (update_hh_loc_total_full \<omega> l v1) l v2 = update_hh_loc_total_full \<omega> l v2"
   sorry
  (* apply (rule full_total_state_eq)
      apply simp
     apply simp
-   apply (simp add: update_heap_total_overwrite)
-  by (metis get_total_full.elims get_mh_total_full.elims snd_conv update_heap_total_full.simps update_heap_total_mask_same)*)
+   apply (simp add: update_hh_loc_total_overwrite)
+  by (metis get_total_full.elims get_mh_total_full.elims snd_conv update_hh_loc_total_full.simps update_hh_loc_total_mask_same)*)
   
-fun update_mask_total_full :: "'a full_total_state \<Rightarrow> mask \<Rightarrow> 'a full_total_state"
-  where "update_mask_total_full \<omega> m = (get_store_total \<omega>, get_trace_total \<omega>, update_mask_total (get_total_full \<omega>) m)"
+fun update_mh_total_full :: "'a full_total_state \<Rightarrow> mask \<Rightarrow> 'a full_total_state"
+  where "update_mh_total_full \<omega> m = (get_store_total \<omega>, get_trace_total \<omega>, update_mh_total (get_total_full \<omega>) m)"
 
-lemma update_heap_total_full_mask_same: "get_mh_total_full (update_heap_total_full \<omega> l v) = get_mh_total_full \<omega>"
-  by (metis get_total_full.simps get_mh_total_full.simps snd_conv update_heap_total_full.simps update_heap_total_mask_same)
+lemma update_hh_loc_total_full_mask_same: "get_mh_total_full (update_hh_loc_total_full \<omega> l v) = get_mh_total_full \<omega>"
+  by (metis get_total_full.simps get_mh_total_full.simps snd_conv update_hh_loc_total_full.simps update_hh_loc_total_mask_same)
 
-lemma get_update_mask_total_full: 
+lemma get_update_mh_total_full: 
   assumes "wf_mask_simple m0"
-  shows   "get_mh_total_full (update_mask_total_full mh m0) = m0"
-  using assms get_update_mask_total
+  shows   "get_mh_total_full (update_mh_total_full mh m0) = m0"
+  using assms get_update_mh_total
   by auto
 
-lemma update_mask_total_full_same:
-  "(update_mask_total_full \<omega> (get_mh_total_full \<omega>)) = \<omega>"
-  by (simp add: update_mask_total_def Rep_total_state_inverse)
+lemma update_mh_total_full_same:
+  "(update_mh_total_full \<omega> (get_mh_total_full \<omega>)) = \<omega>"
+  by (simp add: update_mh_total_def Rep_total_state_inverse)
 
-lemma update_mask_total_same_heap: 
+lemma update_mh_total_same_heap: 
   assumes "wf_mask_simple m"
-  shows "get_hh_total (update_mask_total \<phi> m) = get_hh_total \<phi>"
-  unfolding update_mask_total_def
+  shows "get_hh_total (update_mh_total \<phi> m) = get_hh_total \<phi>"
+  unfolding update_mh_total_def
   using assms
   by (simp add: Abs_total_state_inverse)
 
-lemma update_mask_total_full_same_heap: 
+lemma update_mh_total_full_same_heap: 
   assumes "wf_mask_simple m"
-  shows "get_hh_total_full (update_mask_total_full \<phi> m) = get_hh_total_full \<phi>"
-  using assms update_mask_total_same_heap
+  shows "get_hh_total_full (update_mh_total_full \<phi> m) = get_hh_total_full \<phi>"
+  using assms update_mh_total_same_heap
   by auto
   
-lemma update_mask_total_full_multiple: 
+lemma update_mh_total_full_multiple: 
   assumes "wf_mask_simple m0"
-  shows   "update_mask_total_full (update_mask_total_full \<omega> m0) m1 = update_mask_total_full \<omega> m1"
+  shows   "update_mh_total_full (update_mh_total_full \<omega> m0) m1 = update_mh_total_full \<omega> m1"
   using assms
-  using update_mask_total_multiple by fastforce
+  using update_mh_total_multiple by fastforce
 
-fun update_mask_and_pmask_total_full :: "'a full_total_state \<Rightarrow> mask \<Rightarrow> 'a predicate_mask \<Rightarrow> 'a full_total_state"
-  where "update_mask_and_pmask_total_full \<omega> m pm = 
+fun update_m_total_full :: "'a full_total_state \<Rightarrow> mask \<Rightarrow> 'a predicate_mask \<Rightarrow> 'a full_total_state"
+  where "update_m_total_full \<omega> m pm = 
                 (get_store_total \<omega>, get_trace_total \<omega>, 
-                 update_pmask_total (update_mask_total (get_total_full \<omega>) m) pm)"
+                 update_mp_total (update_mh_total (get_total_full \<omega>) m) pm)"
 
-fun update_pmask_total_full :: "'a full_total_state \<Rightarrow> 'a predicate_mask \<Rightarrow> 'a full_total_state"
-  where "update_pmask_total_full \<omega> pm = (get_store_total \<omega>, get_trace_total \<omega>, update_pmask_total (get_total_full \<omega>) pm)"
+fun update_mp_total_full :: "'a full_total_state \<Rightarrow> 'a predicate_mask \<Rightarrow> 'a full_total_state"
+  where "update_mp_total_full \<omega> pm = (get_store_total \<omega>, get_trace_total \<omega>, update_mp_total (get_total_full \<omega>) pm)"
 
 fun map_result_2 :: "(mask \<Rightarrow> (mask set) option) \<Rightarrow> (mask set) option \<Rightarrow> (mask set) option"
   where 
     "map_result_2 f None = None"
   | "map_result_2 f (Some xs) = (if \<exists>x \<in> xs. f x = None then None else Some (\<Union>x \<in> xs. the (f x))) "
 
+fun map_option_2 :: "('a \<Rightarrow> 'b) \<Rightarrow> 'b \<Rightarrow> 'a option \<Rightarrow> 'b"
+  where 
+    "map_option_2 f y None = y"
+  | "map_option_2 f _ (Some x) = f x"
 
 fun get_address_opt :: "'a val \<Rightarrow> address option"
   where 
