TotalExpressions.thy
@@ -2,18 +2,6 @@ theory TotalExpressions
 imports Viper.ViperLang Viper.ValueAndBasicState TotalViperState Viper.Binop Viper.DeBruijn Viper.PredicatesUtil TotalUtil
 begin
 
-(* duplicated: TODO share it *)
-(*
-fun the_address :: "'a val \<Rightarrow> address" where
-  "the_address (VRef (Address a)) = a"
-| "the_address _ = undefined"
-*)
-
-fun the_rat :: "'a val \<Rightarrow> rat" where
-  "the_rat (VPerm r) = r"
-| "the_rat _ = undefined"
-
-
 fun wd_binop :: "binop \<Rightarrow> 'a val \<Rightarrow> 'a val \<Rightarrow> bool"
   where 
     "wd_binop IntDiv v1 v2 \<longleftrightarrow> v2 \<noteq> (VInt 0)"
@@ -24,23 +12,23 @@ fun wd_binop :: "binop \<Rightarrow> 'a val \<Rightarrow> 'a val \<Rightarrow> b
 datatype 'a standard_result = RMagic | RFailure | RNormal "'a full_total_state"
 
 definition get_valid_locs :: "'a full_total_state \<Rightarrow> heap_loc set"
-  where "get_valid_locs \<omega> = {l |l. pgt (get_mh_total_full \<omega> l) pnone}"
+  where "get_valid_locs \<omega> = {lh |lh. pgt (get_mh_total_full \<omega> lh) pnone}"
 
 
 definition inhale_perm_single :: "'a full_total_state \<Rightarrow> heap_loc \<Rightarrow> prat option \<Rightarrow> 'a full_total_state set"
-  where "inhale_perm_single \<omega> l p_opt =
+  where "inhale_perm_single \<omega> lh p_opt =
       {\<omega>'| \<omega>' q. 
                option_fold ((=) q) (q \<noteq> pnone) p_opt \<and>
-               pgte pwrite (padd (get_mh_total_full \<omega> l) q) \<and>
-               \<omega>' = update_mask_total_full \<omega> ((get_mh_total_full \<omega>)(l := (padd (get_mh_total_full \<omega> l) q)))
+               pgte pwrite (padd (get_mh_total_full \<omega> lh) q) \<and>
+               \<omega>' = update_mh_total_full \<omega> ((get_mh_total_full \<omega>)(lh := (padd (get_mh_total_full \<omega> lh) q)))
        }"
 
 definition inhale_perm_single_pred :: "'a full_total_state \<Rightarrow> 'a predicate_loc \<Rightarrow> prat option \<Rightarrow> 'a full_total_state set"
-  where "inhale_perm_single_pred \<omega> ploc p_opt = 
+  where "inhale_perm_single_pred \<omega> lp p_opt = 
       {\<omega>'| \<omega>' q.   
                option_fold ((=) q) (q \<noteq> pnone) p_opt \<and>
-               pgte pwrite (padd (get_mp_total_full \<omega> ploc) q) \<and>
-               \<omega>' = update_pmask_total_full \<omega> ((get_mp_total_full \<omega>)(ploc := (padd (get_mp_total_full \<omega> ploc) q)))
+               pgte pwrite (padd (get_mp_total_full \<omega> lp) q) \<and>
+               \<omega>' = update_mp_total_full \<omega> ((get_mp_total_full \<omega>)(lp := (padd (get_mp_total_full \<omega> lp) q)))
        }"
 
 fun inh_if_if_total :: "bool \<Rightarrow> bool \<Rightarrow> 'a full_total_state \<Rightarrow> 'a standard_result"  where
@@ -62,41 +50,41 @@ fun sub_expressions_atomic :: "pure_exp atomic_assert \<Rightarrow> pure_exp set
 text\<open>Pure expression evaluation, where the set of heap locations expresses the set of readable locations
 (if no set is provided, then all locations can be read).
 \<close>
-inductive red_pure_exp_total :: "program \<Rightarrow> 'a interp \<Rightarrow> (heap_loc set) option \<Rightarrow> pure_exp \<Rightarrow> 'a full_total_state \<Rightarrow> 'a extended_val \<Rightarrow> bool"
+inductive red_pure_exp_total :: "program \<Rightarrow> 'a interp \<Rightarrow> heap_loc set \<Rightarrow> pure_exp \<Rightarrow> 'a full_total_state \<Rightarrow> 'a extended_val \<Rightarrow> bool"
   ("_, _, _ \<turnstile> ((\<langle>_;_\<rangle>) [\<Down>]\<^sub>t _)" [51,51,51,0,51,51] 81) and
-   red_pure_exps_total :: "program \<Rightarrow> 'a interp \<Rightarrow> (heap_loc set) option \<Rightarrow> pure_exp list \<Rightarrow> 'a full_total_state \<Rightarrow> ('a extended_val) list \<Rightarrow> bool" and
+   red_pure_exps_total :: "program \<Rightarrow> 'a interp \<Rightarrow> heap_loc set \<Rightarrow> pure_exp list \<Rightarrow> 'a full_total_state \<Rightarrow> ('a extended_val) list \<Rightarrow> bool" and
    red_inhale :: "program \<Rightarrow>  'a interp \<Rightarrow> ('a full_total_state \<Rightarrow> bool) \<Rightarrow> assertion \<Rightarrow> 'a full_total_state \<Rightarrow> 'a standard_result \<Rightarrow> bool"
   for Pr :: program and \<Delta> :: "'a interp"
   where
 \<comment>\<open>Atomic inhale\<close>
   InhAcc: 
-    "\<lbrakk> Pr, \<Delta>, Some (get_valid_locs \<omega>) \<turnstile> \<langle>e_r; \<omega>\<rangle> [\<Down>]\<^sub>t Val (VRef r); 
-       Pr, \<Delta>, Some (get_valid_locs \<omega>) \<turnstile> \<langle>e_p; \<omega>\<rangle> [\<Down>]\<^sub>t Val (VPerm p); 
+    "\<lbrakk> Pr, \<Delta>, get_valid_locs \<omega> \<turnstile> \<langle>e_r; \<omega>\<rangle> [\<Down>]\<^sub>t Val (VRef r); 
+       Pr, \<Delta>, get_valid_locs \<omega> \<turnstile> \<langle>e_p; \<omega>\<rangle> [\<Down>]\<^sub>t Val (VPerm p); 
        W' = inhale_perm_single \<omega> (the_address r,f) (Some (Abs_prat p)) \<rbrakk> \<Longrightarrow>
        red_inhale Pr \<Delta> R (Atomic (Acc e_r f (PureExp e_p))) \<omega> 
                 (inh_if_if_total (p \<ge> 0) (W' \<noteq> {} \<and> r \<noteq> Null) (SOME \<omega>'. \<omega>' \<in> W' \<and> R \<omega>'))"
 | InhAccPred:
-    "\<lbrakk> Pr, \<Delta>, Some (get_valid_locs \<omega>) \<turnstile> \<langle>e_p; \<omega>\<rangle> [\<Down>]\<^sub>t Val (VPerm p);
-       red_pure_exps_total Pr \<Delta> (Some (get_valid_locs \<omega>)) e_args \<omega> (map Val v_args);
+    "\<lbrakk> Pr, \<Delta>, get_valid_locs \<omega> \<turnstile> \<langle>e_p; \<omega>\<rangle> [\<Down>]\<^sub>t Val (VPerm p);
+       red_pure_exps_total Pr \<Delta> (get_valid_locs \<omega>) e_args \<omega> (map Val v_args);
        W' = inhale_perm_single_pred \<omega> (pred_id, v_args) (Some (Abs_prat p)) \<rbrakk> \<Longrightarrow>       
        red_inhale Pr \<Delta> R (Atomic (AccPredicate pred_id e_args (PureExp e_p))) \<omega> 
                 (inh_if_if_total (p \<ge> 0) (W' \<noteq> {} \<and> r \<noteq> Null) (SOME \<omega>'. \<omega>' \<in> W' \<and> R \<omega>'))"
 | InhAccWildcard: 
-    "\<lbrakk> Pr, \<Delta>, Some (get_valid_locs \<omega>) \<turnstile> \<langle>e_r; \<omega>\<rangle> [\<Down>]\<^sub>t Val (VRef r);
+    "\<lbrakk> Pr, \<Delta>, get_valid_locs \<omega> \<turnstile> \<langle>e_r; \<omega>\<rangle> [\<Down>]\<^sub>t Val (VRef r);
        W' = inhale_perm_single \<omega> (the_address r,f) None \<rbrakk> \<Longrightarrow>
        red_inhale Pr \<Delta> R (Atomic (Acc e_r f Wildcard)) \<omega> 
                    (inh_if_if_total True (W' \<noteq> {} \<and> r \<noteq> Null) (SOME \<omega>'. \<omega>' \<in> W' \<and> R \<omega>'))"
 | InhAccPredWildcard: 
-    "\<lbrakk> Pr, \<Delta>, Some (get_valid_locs \<omega>) \<turnstile> \<langle>e_r; \<omega>\<rangle> [\<Down>]\<^sub>t Val (VRef r);
+    "\<lbrakk> Pr, \<Delta>, get_valid_locs \<omega> \<turnstile> \<langle>e_r; \<omega>\<rangle> [\<Down>]\<^sub>t Val (VRef r);
        W' = inhale_perm_single_pred \<omega> (pred_id, v_args) None \<rbrakk> \<Longrightarrow>
        red_inhale Pr \<Delta> R (Atomic (AccPredicate pred_id e_args Wildcard)) \<omega> 
                  (inh_if_if_total True (W' \<noteq> {} \<and> r \<noteq> Null) (SOME \<omega>'. \<omega>' \<in> W' \<and> R \<omega>'))"
 | InhPureNormalMagic: 
-    "\<lbrakk> Pr, \<Delta>, Some (get_valid_locs \<omega>) \<turnstile> \<langle>e; \<omega>\<rangle> [\<Down>]\<^sub>t Val (VBool b) \<rbrakk> \<Longrightarrow>
+    "\<lbrakk> Pr, \<Delta>, get_valid_locs \<omega> \<turnstile> \<langle>e; \<omega>\<rangle> [\<Down>]\<^sub>t Val (VBool b) \<rbrakk> \<Longrightarrow>
       red_inhale Pr \<Delta> R (Atomic (Pure e)) \<omega> (if b then RNormal \<omega> else RMagic)"
 | SubFailure: 
-    "\<lbrakk> e \<in> sub_expressions_atomic A; Pr, \<Delta>, Some (get_valid_locs \<omega>) \<turnstile> \<langle>e; \<omega>\<rangle> [\<Down>]\<^sub>t VFailure \<rbrakk> \<Longrightarrow> 
-      red_inhale Pr \<Delta>  R (Atomic A) \<omega> RFailure"
+    "\<lbrakk> e \<in> sub_expressions_atomic A; Pr, \<Delta>, get_valid_locs \<omega> \<turnstile> \<langle>e; \<omega>\<rangle> [\<Down>]\<^sub>t VFailure \<rbrakk> \<Longrightarrow> 
+      red_inhale Pr \<Delta> R (Atomic A) \<omega> RFailure"
 
 \<comment>\<open>Connectives inhale\<close>
 | InhSepNormal: 
@@ -109,70 +97,70 @@ inductive red_pure_exp_total :: "program \<Rightarrow> 'a interp \<Rightarrow> (
       red_inhale Pr \<Delta> R (A && B) \<omega> resA"
 | InhImpTrue:
  "\<lbrakk> 
-    Pr, \<Delta>, Some (get_valid_locs \<omega>) \<turnstile> \<langle>e; \<omega>\<rangle> [\<Down>]\<^sub>t (Val (VBool True)); 
+    Pr, \<Delta>, get_valid_locs \<omega> \<turnstile> \<langle>e; \<omega>\<rangle> [\<Down>]\<^sub>t (Val (VBool True)); 
     red_inhale Pr \<Delta> R A \<omega> res \<rbrakk> \<Longrightarrow>
     red_inhale Pr \<Delta> R (Imp e A) \<omega> res"
 | InhImpFalse:
- "\<lbrakk> Pr, \<Delta>, Some (get_valid_locs \<omega>) \<turnstile> \<langle>e; \<omega>\<rangle> [\<Down>]\<^sub>t Val (VBool False) \<rbrakk> \<Longrightarrow> 
+ "\<lbrakk> Pr, \<Delta>, get_valid_locs \<omega> \<turnstile> \<langle>e; \<omega>\<rangle> [\<Down>]\<^sub>t Val (VBool False) \<rbrakk> \<Longrightarrow> 
     red_inhale Pr \<Delta> R (Imp e A) \<omega> (RNormal \<omega>)"
 | InhImpFailure:
- "\<lbrakk> Pr, \<Delta>, Some (get_valid_locs \<omega>) \<turnstile> \<langle>e; \<omega>\<rangle> [\<Down>]\<^sub>t VFailure \<rbrakk> \<Longrightarrow>
+ "\<lbrakk> Pr, \<Delta>, get_valid_locs \<omega> \<turnstile> \<langle>e; \<omega>\<rangle> [\<Down>]\<^sub>t VFailure \<rbrakk> \<Longrightarrow>
    red_inhale Pr \<Delta> R (Imp e A) \<omega> RFailure"
 
 \<comment>\<open>Pure expression evaluation\<close>
 
 
 \<comment>\<open>Atomic expressions\<close>
-| RedLit: "Pr, \<Delta>, HLOpt \<turnstile> \<langle>ELit l; _\<rangle> [\<Down>]\<^sub>t Val (val_of_lit l)"
-| RedVar: "\<lbrakk> \<sigma> n = Some v \<rbrakk> \<Longrightarrow> Pr, \<Delta>, HLOpt \<turnstile> \<langle>Var n; (\<sigma>, _, _)\<rangle> [\<Down>]\<^sub>t Val v"
-| RedResult: "\<lbrakk> \<sigma> 0 = Some v \<rbrakk> \<Longrightarrow> Pr, \<Delta>, HLOpt \<turnstile> \<langle>Result; (\<sigma>, _, _)\<rangle> [\<Down>]\<^sub>t Val v"
+| RedLit: "Pr, \<Delta>, LH \<turnstile> \<langle>ELit l; _\<rangle> [\<Down>]\<^sub>t Val (val_of_lit l)"
+| RedVar: "\<lbrakk> \<sigma> n = Some v \<rbrakk> \<Longrightarrow> Pr, \<Delta>, LH \<turnstile> \<langle>Var n; (\<sigma>, _, _)\<rangle> [\<Down>]\<^sub>t Val v"
+| RedResult: "\<lbrakk> \<sigma> 0 = Some v \<rbrakk> \<Longrightarrow> Pr, \<Delta>, LH \<turnstile> \<langle>Result; (\<sigma>, _, _)\<rangle> [\<Down>]\<^sub>t Val v"
 
 \<comment>\<open>Binop and Unop\<close>
-| RedBinopLazy: "\<lbrakk> Pr, \<Delta>, HLOpt \<turnstile> \<langle>e1; \<omega>\<rangle> [\<Down>]\<^sub>t Val v1 ; eval_binop_lazy v1 bop = Some v \<rbrakk>
-  \<Longrightarrow> Pr, \<Delta>, HLOpt \<turnstile> \<langle>Binop e1 bop e2; \<omega>\<rangle> [\<Down>]\<^sub>t Val v"
-| RedBinop: "\<lbrakk> Pr, \<Delta>, HLOpt \<turnstile> \<langle>e1; \<omega>\<rangle> [\<Down>]\<^sub>t Val v1 ; Pr, \<Delta>, HLOpt \<turnstile> \<langle>e2; \<omega>\<rangle> [\<Down>]\<^sub>t Val v2 ; eval_binop_lazy v1 bop = None; eval_binop v1 bop v2 = BinopNormal v \<rbrakk>
-  \<Longrightarrow> Pr, \<Delta>, HLOpt \<turnstile> \<langle>Binop e1 bop e2; \<omega>\<rangle> [\<Down>]\<^sub>t Val v"
-| RedBinopRightFailure: "\<lbrakk> Pr, \<Delta>, HLOpt \<turnstile> \<langle>e1; \<omega>\<rangle> [\<Down>]\<^sub>t Val v1; Pr, \<Delta>, HLOpt \<turnstile> \<langle>e2; \<omega>\<rangle> [\<Down>]\<^sub>t VFailure;  eval_binop_lazy v1 bop = None \<rbrakk>
-  \<Longrightarrow> Pr, \<Delta>, HLOpt \<turnstile> \<langle>Binop e1 bop e2; \<omega>\<rangle> [\<Down>]\<^sub>t VFailure"
-| RedBinopOpFailure: "\<lbrakk> Pr, \<Delta>, HLOpt \<turnstile> \<langle>e1; \<omega>\<rangle> [\<Down>]\<^sub>t Val v1 ; Pr, \<Delta>, HLOpt \<turnstile> \<langle>e2; \<omega>\<rangle> [\<Down>]\<^sub>t Val v2 ; eval_binop v1 bop v2 = BinopOpFailure ; eval_binop_lazy v1 bop = None \<rbrakk>
-  \<Longrightarrow> Pr, \<Delta>, HLOpt \<turnstile> \<langle>Binop e1 bop e2; \<omega>\<rangle> [\<Down>]\<^sub>t VFailure" (* Division by 0 *)
-| RedBinopLeftFailure: "\<lbrakk> Pr, \<Delta>, HLOpt \<turnstile> \<langle>e1; \<omega>\<rangle> [\<Down>]\<^sub>t VFailure \<rbrakk>
-  \<Longrightarrow> Pr, \<Delta>, HLOpt \<turnstile> \<langle>Binop e1 bop e2; \<omega>\<rangle> [\<Down>]\<^sub>t VFailure" (* could be replaced *)
+| RedBinopLazy: "\<lbrakk> Pr, \<Delta>, LH \<turnstile> \<langle>e1; \<omega>\<rangle> [\<Down>]\<^sub>t Val v1 ; eval_binop_lazy v1 bop = Some v \<rbrakk>
+  \<Longrightarrow> Pr, \<Delta>, LH \<turnstile> \<langle>Binop e1 bop e2; \<omega>\<rangle> [\<Down>]\<^sub>t Val v"
+| RedBinop: "\<lbrakk> Pr, \<Delta>, LH \<turnstile> \<langle>e1; \<omega>\<rangle> [\<Down>]\<^sub>t Val v1 ; Pr, \<Delta>, LH \<turnstile> \<langle>e2; \<omega>\<rangle> [\<Down>]\<^sub>t Val v2 ; eval_binop_lazy v1 bop = None; eval_binop v1 bop v2 = BinopNormal v \<rbrakk>
+  \<Longrightarrow> Pr, \<Delta>, LH \<turnstile> \<langle>Binop e1 bop e2; \<omega>\<rangle> [\<Down>]\<^sub>t Val v"
+| RedBinopRightFailure: "\<lbrakk> Pr, \<Delta>, LH \<turnstile> \<langle>e1; \<omega>\<rangle> [\<Down>]\<^sub>t Val v1; Pr, \<Delta>, LH \<turnstile> \<langle>e2; \<omega>\<rangle> [\<Down>]\<^sub>t VFailure;  eval_binop_lazy v1 bop = None \<rbrakk>
+  \<Longrightarrow> Pr, \<Delta>, LH \<turnstile> \<langle>Binop e1 bop e2; \<omega>\<rangle> [\<Down>]\<^sub>t VFailure"
+| RedBinopOpFailure: "\<lbrakk> Pr, \<Delta>, LH \<turnstile> \<langle>e1; \<omega>\<rangle> [\<Down>]\<^sub>t Val v1 ; Pr, \<Delta>, LH \<turnstile> \<langle>e2; \<omega>\<rangle> [\<Down>]\<^sub>t Val v2 ; eval_binop v1 bop v2 = BinopOpFailure ; eval_binop_lazy v1 bop = None \<rbrakk>
+  \<Longrightarrow> Pr, \<Delta>, LH \<turnstile> \<langle>Binop e1 bop e2; \<omega>\<rangle> [\<Down>]\<^sub>t VFailure" (* Division by 0 *)
+| RedBinopLeftFailure: "\<lbrakk> Pr, \<Delta>, LH \<turnstile> \<langle>e1; \<omega>\<rangle> [\<Down>]\<^sub>t VFailure \<rbrakk>
+  \<Longrightarrow> Pr, \<Delta>, LH \<turnstile> \<langle>Binop e1 bop e2; \<omega>\<rangle> [\<Down>]\<^sub>t VFailure" (* could be replaced *)
 
-| RedUnop: "\<lbrakk> Pr, \<Delta>, HLOpt \<turnstile> \<langle>e; \<omega>\<rangle> [\<Down>]\<^sub>t Val v; eval_unop unop v = BinopNormal v' \<rbrakk> \<Longrightarrow> Pr, \<Delta>, HLOpt \<turnstile> \<langle>Unop unop e; \<omega>\<rangle> [\<Down>]\<^sub>t Val v'"
-| RedUnopFailure: "\<lbrakk> Pr, \<Delta>, HLOpt \<turnstile> \<langle>e; \<omega>\<rangle> [\<Down>]\<^sub>t VFailure \<rbrakk> \<Longrightarrow> Pr, \<Delta>, HLOpt \<turnstile> \<langle>Unop unop e; \<omega>\<rangle> [\<Down>]\<^sub>t VFailure" (* could be replaced *)
+| RedUnop: "\<lbrakk> Pr, \<Delta>, LH \<turnstile> \<langle>e; \<omega>\<rangle> [\<Down>]\<^sub>t Val v; eval_unop unop v = BinopNormal v' \<rbrakk> \<Longrightarrow> Pr, \<Delta>, LH \<turnstile> \<langle>Unop unop e; \<omega>\<rangle> [\<Down>]\<^sub>t Val v'"
+| RedUnopFailure: "\<lbrakk> Pr, \<Delta>, LH \<turnstile> \<langle>e; \<omega>\<rangle> [\<Down>]\<^sub>t VFailure \<rbrakk> \<Longrightarrow> Pr, \<Delta>, LH \<turnstile> \<langle>Unop unop e; \<omega>\<rangle> [\<Down>]\<^sub>t VFailure" (* could be replaced *)
 
 \<comment>\<open>Cond\<close>
-| RedCondExpTrue: "\<lbrakk> Pr, \<Delta>, HLOpt \<turnstile> \<langle>e1; \<omega>\<rangle> [\<Down>]\<^sub>t Val (VBool True) ; Pr, \<Delta>, HLOpt \<turnstile> \<langle>e2; \<omega>\<rangle> [\<Down>]\<^sub>t r \<rbrakk>
-  \<Longrightarrow> Pr, \<Delta>, HLOpt \<turnstile> \<langle>CondExp e1 e2 e3; \<omega>\<rangle> [\<Down>]\<^sub>t r"
-| RedCondExpFalse: "\<lbrakk> Pr, \<Delta>, HLOpt \<turnstile> \<langle>e1; \<omega>\<rangle> [\<Down>]\<^sub>t Val (VBool False) ; Pr, \<Delta>, HLOpt \<turnstile> \<langle>e3; \<omega>\<rangle> [\<Down>]\<^sub>t r \<rbrakk>
-  \<Longrightarrow> Pr, \<Delta>, HLOpt \<turnstile> \<langle>CondExp e1 e2 e3; \<omega>\<rangle> [\<Down>]\<^sub>t r"
-| RedCondExpFailure: "\<lbrakk> Pr, \<Delta>, HLOpt \<turnstile> \<langle>e1; \<omega>\<rangle> [\<Down>]\<^sub>t VFailure \<rbrakk>
-  \<Longrightarrow> Pr, \<Delta>, HLOpt \<turnstile> \<langle>CondExp e1 e2 e3; \<omega>\<rangle> [\<Down>]\<^sub>t VFailure" (* could be replaced *)
+| RedCondExpTrue: "\<lbrakk> Pr, \<Delta>, LH \<turnstile> \<langle>e1; \<omega>\<rangle> [\<Down>]\<^sub>t Val (VBool True) ; Pr, \<Delta>, LH \<turnstile> \<langle>e2; \<omega>\<rangle> [\<Down>]\<^sub>t r \<rbrakk>
+  \<Longrightarrow> Pr, \<Delta>, LH \<turnstile> \<langle>CondExp e1 e2 e3; \<omega>\<rangle> [\<Down>]\<^sub>t r"
+| RedCondExpFalse: "\<lbrakk> Pr, \<Delta>, LH \<turnstile> \<langle>e1; \<omega>\<rangle> [\<Down>]\<^sub>t Val (VBool False) ; Pr, \<Delta>, LH \<turnstile> \<langle>e3; \<omega>\<rangle> [\<Down>]\<^sub>t r \<rbrakk>
+  \<Longrightarrow> Pr, \<Delta>, LH \<turnstile> \<langle>CondExp e1 e2 e3; \<omega>\<rangle> [\<Down>]\<^sub>t r"
+| RedCondExpFailure: "\<lbrakk> Pr, \<Delta>, LH \<turnstile> \<langle>e1; \<omega>\<rangle> [\<Down>]\<^sub>t VFailure \<rbrakk>
+  \<Longrightarrow> Pr, \<Delta>, LH \<turnstile> \<langle>CondExp e1 e2 e3; \<omega>\<rangle> [\<Down>]\<^sub>t VFailure" (* could be replaced *)
 
 \<comment>\<open>Old\<close>
-| RedOld: "\<lbrakk> t l = Some \<phi> ; Pr, \<Delta>, HLOpt \<turnstile> \<langle>e; (\<sigma>, t, \<phi>)\<rangle> [\<Down>]\<^sub>t v \<rbrakk> \<Longrightarrow> Pr, \<Delta>, HLOpt \<turnstile> \<langle>Old l e; (\<sigma>, t, _)\<rangle> [\<Down>]\<^sub>t v"
-| RedOldFailure: "\<lbrakk> t l = None \<rbrakk> \<Longrightarrow> Pr, \<Delta>, HLOpt \<turnstile> \<langle>Old l e ; (_, t, _)\<rangle> [\<Down>]\<^sub>t VFailure" 
+| RedOld: "\<lbrakk> t l = Some \<phi> ; Pr, \<Delta>, LH \<turnstile> \<langle>e; (\<sigma>, t, \<phi>)\<rangle> [\<Down>]\<^sub>t v \<rbrakk> \<Longrightarrow> Pr, \<Delta>, LH \<turnstile> \<langle>Old l e; (\<sigma>, t, _)\<rangle> [\<Down>]\<^sub>t v"
+| RedOldFailure: "\<lbrakk> t l = None \<rbrakk> \<Longrightarrow> Pr, \<Delta>, LH \<turnstile> \<langle>Old l e ; (_, t, _)\<rangle> [\<Down>]\<^sub>t VFailure" 
 
 \<comment>\<open>Heap lookup\<close>
-| RedField: "\<lbrakk> Pr, \<Delta>, HLOpt \<turnstile> \<langle>e; \<omega>\<rangle> [\<Down>]\<^sub>t Val (VRef (Address a)) ; get_heap_total_full \<omega> (a, f) = v \<rbrakk> \<Longrightarrow> 
-       Pr, \<Delta>, HLOpt \<turnstile> \<langle>FieldAcc e f; \<omega>\<rangle> [\<Down>]\<^sub>t option_fold (\<lambda>l. if (a,f) \<in> l then Val v else VFailure) (Val v) HLOpt"
-| RedFieldFailure: "\<lbrakk> Pr, \<Delta>, HLOpt \<turnstile> \<langle>e; \<omega>\<rangle> [\<Down>]\<^sub>t VFailure \<rbrakk> \<Longrightarrow> Pr, \<Delta>, HLOpt \<turnstile> \<langle>FieldAcc e f; \<omega>\<rangle> [\<Down>]\<^sub>t VFailure" (* could be replaced *)
+| RedField: "\<lbrakk> Pr, \<Delta>, LH \<turnstile> \<langle>e; \<omega>\<rangle> [\<Down>]\<^sub>t Val (VRef (Address a)) ; get_hh_total_full \<omega> (a, f) = v \<rbrakk> \<Longrightarrow> 
+       Pr, \<Delta>, LH \<turnstile> \<langle>FieldAcc e f; \<omega>\<rangle> [\<Down>]\<^sub>t (if (a,f) \<in> LH then Val v else VFailure)"
+| RedFieldFailure: "\<lbrakk> Pr, \<Delta>, LH \<turnstile> \<langle>e; \<omega>\<rangle> [\<Down>]\<^sub>t VFailure \<rbrakk> \<Longrightarrow> Pr, \<Delta>, LH \<turnstile> \<langle>FieldAcc e f; \<omega>\<rangle> [\<Down>]\<^sub>t VFailure" (* could be replaced *)
 
 \<comment>\<open>Permission introspection\<close>
-| RedPermNull: "\<lbrakk> Pr, \<Delta>, HLOpt \<turnstile> \<langle>e; \<omega>\<rangle> [\<Down>]\<^sub>t Val (VRef Null) \<rbrakk> \<Longrightarrow> Pr, \<Delta>, HLOpt \<turnstile> \<langle>Perm e f; \<omega>\<rangle> [\<Down>]\<^sub>t Val (VPerm 0)"
-| RedPerm: "\<lbrakk> Pr, \<Delta>, HLOpt \<turnstile> \<langle>e; \<omega>\<rangle> [\<Down>]\<^sub>t Val (VRef (Address a)) \<rbrakk> \<Longrightarrow> Pr, \<Delta>, HLOpt \<turnstile> \<langle>Perm e f; \<omega>\<rangle> [\<Down>]\<^sub>t Val (VPerm (Rep_prat (get_mask_total_full \<omega> (a, f))))"
-| RedPermFailure: "\<lbrakk> Pr, \<Delta>, HLOpt \<turnstile> \<langle>e; \<omega>\<rangle> [\<Down>]\<^sub>t VFailure \<rbrakk> \<Longrightarrow> Pr, \<Delta>, HLOpt \<turnstile> \<langle>Perm e f; \<omega>\<rangle> [\<Down>]\<^sub>t VFailure" (* could be replaced *)
+| RedPermNull: "\<lbrakk> Pr, \<Delta>, LH \<turnstile> \<langle>e; \<omega>\<rangle> [\<Down>]\<^sub>t Val (VRef Null) \<rbrakk> \<Longrightarrow> Pr, \<Delta>, LH \<turnstile> \<langle>Perm e f; \<omega>\<rangle> [\<Down>]\<^sub>t Val (VPerm 0)"
+| RedPerm: "\<lbrakk> Pr, \<Delta>, LH \<turnstile> \<langle>e; \<omega>\<rangle> [\<Down>]\<^sub>t Val (VRef (Address a)) \<rbrakk> \<Longrightarrow> Pr, \<Delta>, LH \<turnstile> \<langle>Perm e f; \<omega>\<rangle> [\<Down>]\<^sub>t Val (VPerm (Rep_prat (get_mh_total_full \<omega> (a, f))))"
+| RedPermFailure: "\<lbrakk> Pr, \<Delta>, LH \<turnstile> \<langle>e; \<omega>\<rangle> [\<Down>]\<^sub>t VFailure \<rbrakk> \<Longrightarrow> Pr, \<Delta>, LH \<turnstile> \<langle>Perm e f; \<omega>\<rangle> [\<Down>]\<^sub>t VFailure" (* could be replaced *)
 (*
 \<comment>\<open>Unfolding\<close>
 | RedUnfolding: "\<lbrakk> 
-         Pr, \<Delta>, HLOpt \<turnstile> \<langle>e_arg; \<omega>\<rangle> [\<Down>]\<^sub>t v_arg;
+         Pr, \<Delta>, LH \<turnstile> \<langle>e_arg; \<omega>\<rangle> [\<Down>]\<^sub>t v_arg;
         ViperLang.predicates Pr p = Some pred;
         ViperLang.predicate_decl.body pred = Some pred_body;
         red_inhale Pr \<Delta> False pred_body \<omega> (RNormal \<omega>');
             
  \<rbrakk> \<Longrightarrow>
-     Pr, \<Delta>, HLOpt \<turnstile> \<langle>Unfolding p [e_arg] p_body; \<omega>\<rangle> [\<Down>]\<^sub>t Val (VPerm 0)"
+     Pr, \<Delta>, LH \<turnstile> \<langle>Unfolding p [e_arg] p_body; \<omega>\<rangle> [\<Down>]\<^sub>t Val (VPerm 0)"
 *)
 
 (*| RedPropagateFailure: "\<lbrakk> e \<in> sub_pure_exp e' ; Pr, \<Delta> \<turnstile> \<langle>e; \<omega>\<rangle> [\<Down>]\<^sub>t VFailure \<rbrakk> \<Longrightarrow>  Pr, \<Delta> \<turnstile> \<langle>e'; \<omega>\<rangle> [\<Down>]\<^sub>t VFailure"*)
@@ -204,7 +192,7 @@ inductive unfold_rel :: "program \<Rightarrow> 'a interp \<Rightarrow> predicate
   where UnfoldRelStep: 
                     "\<lbrakk> ViperLang.predicates Pr pred_id = Some pred_decl;
                      ViperLang.predicate_decl.body pred_decl = Some pred_body;
-                     m = get_pmask_total_full \<omega>;
+                     m = get_mp_total_full \<omega>;
                      pgte (m (pred_id,vs)) q;
                      m' = m( (pred_id,vs) := psub (m (pred_id, vs)) q);
                      \<omega>2 = (nth_option vs, get_trace_total \<omega>, update_pmask_total (get_mh_total_full \<omega>) m');
@@ -219,7 +207,7 @@ definition unfold_rel_multi
 
 coinductive unfold_consistent :: "program \<Rightarrow> 'a interp \<Rightarrow> 'a full_total_state \<Rightarrow> bool"
   where 
-  unfold_step: "\<lbrakk> \<And> pred_id vs q. pgt (get_pmask_total_full \<omega> (pred_id,vs)) q \<Longrightarrow>
+  unfold_step: "\<lbrakk> \<And> pred_id vs q. pgt (get_mp_total_full \<omega> (pred_id,vs)) q \<Longrightarrow>
                      \<exists>\<omega>'. unfold_rel Pr \<Delta> pred_id vs q \<omega> \<omega>' \<and> unfold_consistent Pr \<Delta> \<omega>' \<rbrakk> \<Longrightarrow>
                   unfold_consistent Pr \<Delta> \<omega>"
 
@@ -227,23 +215,27 @@ coinductive unfold_consistent :: "program \<Rightarrow> 'a interp \<Rightarrow> 
 definition unfold_consistent where
  "unfold_consistent Pr \<Delta> \<omega> \<equiv> 
           \<forall> \<omega>' pred_id vs q. 
-               (unfold_rel_multi Pr \<Delta> \<omega> \<omega>' \<and> pgt (get_pmask_total_full \<omega>' (pred_id,vs)) q) \<longrightarrow>
+               (unfold_rel_multi Pr \<Delta> \<omega> \<omega>' \<and> pgt (get_mp_total_full \<omega>' (pred_id,vs)) q) \<longrightarrow>
                (\<exists>\<omega>''. unfold_rel Pr \<Delta> pred_id vs q \<omega>' \<omega>'')"
 *)
 
 text \<open>Expression evaluation as a function. Using this function makes sense, when it is known that 
-e is well-defined and is deterministic (for example, if e is the body of a predicate)\<close>
+e is well-defined and is deterministic (for example, if e is the body of a predicate). \<^term>\<open>UNIV\<close>
+is used to indicate that every heap location can be read (effectively omitting heap checks)\<close>
+
 fun red_pure_exp_total_fun :: "program \<Rightarrow> 'a interp \<Rightarrow> pure_exp \<Rightarrow> 'a full_total_state \<Rightarrow> 'a val"
-  where "red_pure_exp_total_fun Pr \<Delta> e \<omega> = (SOME v. Pr, \<Delta>, None \<turnstile> \<langle>e; \<omega>\<rangle> [\<Down>]\<^sub>t Val v)"
+  where "red_pure_exp_total_fun Pr \<Delta> e \<omega> = (SOME v. Pr, \<Delta>, UNIV \<turnstile> \<langle>e; \<omega>\<rangle> [\<Down>]\<^sub>t Val v)"
 
 fun red_pure_exps_total_fun :: "program \<Rightarrow> 'a interp \<Rightarrow> pure_exp list \<Rightarrow> 'a full_total_state \<Rightarrow> ('a val) list"
-  where "red_pure_exps_total_fun Pr \<Delta> es \<omega> = (SOME vs. red_pure_exps_total Pr \<Delta> None es \<omega> (map Val vs))"
+  where "red_pure_exps_total_fun Pr \<Delta> es \<omega> = (SOME vs. red_pure_exps_total Pr \<Delta> UNIV es \<omega> (map Val vs))"
 
+(* TODO: duplicate? *)
 fun extract_address_from_val :: "'a val \<Rightarrow> address"
   where 
     "extract_address_from_val (VRef (Address a)) = a"
   | "extract_address_from_val _ = undefined"
 
+(* TODO: duplicate? *)
 fun extract_perm_from_val :: "'a val \<Rightarrow> rat"
   where 
     "extract_perm_from_val (VPerm r) = r"
@@ -264,7 +256,7 @@ fun assertion_heap_snapshot :: "program \<Rightarrow> 'a interp \<Rightarrow> as
               else {})"
  | "assertion_heap_snapshot Pr \<Delta> (Atomic (AccPredicate pred_id e_args e_p)) \<omega> = 
              (if is_positive_permission Pr \<Delta> e_p \<omega> then
-                fst (get_pheap_total_full \<omega> (pred_id, red_pure_exps_total_fun Pr \<Delta> e_args \<omega>))
+                fst (get_hp_total_full \<omega> (pred_id, red_pure_exps_total_fun Pr \<Delta> e_args \<omega>))
               else {})"
  | "assertion_heap_snapshot Pr \<Delta> (Imp e A) \<omega> =
              (if red_pure_exp_total_fun Pr \<Delta> e \<omega> = VBool True then 
@@ -280,7 +272,7 @@ fun assertion_predicate_snapshot :: "program \<Rightarrow> 'a interp \<Rightarro
  | "assertion_predicate_snapshot Pr \<Delta> (Atomic (AccPredicate pred_id e_args e_p)) \<omega> = 
              (if is_positive_permission Pr \<Delta> e_p \<omega> then
                 {(pred_id, red_pure_exps_total_fun Pr \<Delta> e_args \<omega>)} \<union> 
-                snd (get_pheap_total_full \<omega> (pred_id, red_pure_exps_total_fun Pr \<Delta> e_args \<omega>))
+                snd (get_hp_total_full \<omega> (pred_id, red_pure_exps_total_fun Pr \<Delta> e_args \<omega>))
               else {})"
  | "assertion_predicate_snapshot Pr \<Delta> (Imp e A) \<omega> =
              (if red_pure_exp_total_fun Pr \<Delta> e \<omega> = VBool True then 
@@ -293,17 +285,25 @@ fun assertion_predicate_snapshot :: "program \<Rightarrow> 'a interp \<Rightarro
 definition pheap_consistent :: "program \<Rightarrow> 'a interp \<Rightarrow> 'a full_total_state \<Rightarrow> bool" where
  "pheap_consistent Pr \<Delta> \<omega> \<equiv> 
           \<forall> \<omega>' pred_id vs pred_decl. 
-               (unfold_rel_multi Pr \<Delta> \<omega> \<omega>' \<and> pgt (get_pmask_total_full \<omega>' (pred_id,vs)) pnone \<and>
+               (unfold_rel_multi Pr \<Delta> \<omega> \<omega>' \<and> pgt (get_mp_total_full \<omega>' (pred_id,vs)) pnone \<and>
                 ViperLang.predicates Pr pred_id = Some pred_decl) \<longrightarrow>
-                option_fold (\<lambda> pred_body. get_pheap_total_full \<omega> (pred_id, vs) = 
+                option_fold (\<lambda> pred_body. get_hp_total_full \<omega> (pred_id, vs) = 
                               (assertion_heap_snapshot Pr \<Delta> pred_body \<omega>, assertion_predicate_snapshot Pr \<Delta> pred_body \<omega>) )
                             True
                             (ViperLang.predicate_decl.body pred_decl)"
 
+definition total_heap_consistent :: "program \<Rightarrow> 'a interp \<Rightarrow> 'a full_total_state \<Rightarrow> bool"
+  where "total_heap_consistent Pr \<Delta> \<omega> \<equiv> unfold_consistent Pr \<Delta> \<omega> \<and> pheap_consistent Pr \<Delta> \<omega>"
 
 
-datatype inh_exh_conf = CInhale | CExhale "heap_loc set"
+abbreviation red_inhale1 :: "program \<Rightarrow> 'a interp \<Rightarrow> assertion \<Rightarrow> 'a full_total_state \<Rightarrow> 'a standard_result \<Rightarrow> bool"
+  where "red_inhale1 Pr \<Delta> A \<omega> res \<equiv> red_inhale Pr \<Delta> (total_heap_consistent Pr \<Delta>) A \<omega> res"
+
+text \<open>\<^const>\<open>red_inhale1\<close> only takes transitions to total heap consistent states whenever some permission is inhaled\<close>
+
 (*
+datatype inh_exh_conf = CInhale | CExhale "heap_loc set"
+
 (* can't show this, since need to take typing into account *)
 lemma wd_binop_total: 
   assumes "wd_binop bop v1 v2"
@@ -321,7 +321,7 @@ fun wd_pure_exp_total :: "program \<Rightarrow> 'a interp \<Rightarrow> inh_exh_
 | "wd_pure_exp_total Pr \<Delta> c (CondExp e1 e2 e3) \<omega> \<longleftrightarrow> 
      wd_pure_exp_total Pr \<Delta> c e1 \<omega> \<and> (if ((Pr,\<Delta> \<turnstile> \<langle>e1; \<omega>\<rangle> [\<Down>]\<^sub>t Val (VBool True))) then wd_pure_exp_total Pr \<Delta> c e2 \<omega> else wd_pure_exp_total Pr \<Delta> c e3 \<omega>)" 
 | "wd_pure_exp_total Pr \<Delta> CInhale (FieldAcc e f) \<omega> \<longleftrightarrow> 
-    wd_pure_exp_total Pr \<Delta> CInhale e \<omega> \<and> (\<forall>l. (Pr, \<Delta> \<turnstile> \<langle>e;\<omega>\<rangle> [\<Down>]\<^sub>t Val (VRef (Address l))) \<longrightarrow> (pgt (get_mask_total_full \<omega> (l,f)) pnone))"
+    wd_pure_exp_total Pr \<Delta> CInhale e \<omega> \<and> (\<forall>l. (Pr, \<Delta> \<turnstile> \<langle>e;\<omega>\<rangle> [\<Down>]\<^sub>t Val (VRef (Address l))) \<longrightarrow> (pgt (get_mh_total_full \<omega> (l,f)) pnone))"
 | "wd_pure_exp_total Pr \<Delta> (CExhale locs) (FieldAcc e f) \<omega> \<longleftrightarrow> 
     wd_pure_exp_total Pr \<Delta> (CExhale locs) e \<omega> \<and>
     (\<forall>l. ( (Pr,\<Delta> \<turnstile> \<langle>e;\<omega>\<rangle> [\<Down>]\<^sub>t Val (VRef (Address l))) \<longrightarrow> (l,f) \<in> locs))"
