TotalSemantics.thy
@@ -22,11 +22,11 @@ fun exh_if_total :: "bool \<Rightarrow> mask \<times> 'a predicate_mask \<Righta
 
 
 definition exhale_perm_single :: "mask \<Rightarrow> heap_loc \<Rightarrow> prat option \<Rightarrow> mask set"
-  where "exhale_perm_single m l p_opt =
+  where "exhale_perm_single m lh p_opt =
       {m'| m' q. 
                (p_opt = None \<longrightarrow> pgt q pnone) \<and>
-               option_fold ((=) q) (q \<noteq> pnone \<and> pgt (m l) q) p_opt \<and>
-               m' = m(l := psub (m l) q)
+               option_fold ((=) q) (q \<noteq> pnone \<and> pgt (m lh) q) p_opt \<and>
+               m' = m(lh := psub (m lh) q)
        }"
 
 
@@ -36,17 +36,17 @@ inductive red_exhale :: "program \<Rightarrow> 'a interp \<Rightarrow> 'a full_t
 
 \<comment>\<open>exhale acc(e.f, p)\<close>
     ExhAcc: 
-    "\<lbrakk> \<omega> = update_mask_total_full \<omega>0 m;
-       Pr, \<Delta>, Some (get_valid_locs \<omega>0) \<turnstile> \<langle>e_r; \<omega>\<rangle> [\<Down>]\<^sub>t Val (VRef r); 
-       Pr, \<Delta>, Some (get_valid_locs \<omega>0) \<turnstile> \<langle>e_p; \<omega>\<rangle> [\<Down>]\<^sub>t Val (VPerm p);
+    "\<lbrakk> \<omega> = update_mh_total_full \<omega>0 m;
+       Pr, \<Delta>, get_valid_locs \<omega>0 \<turnstile> \<langle>e_r; \<omega>\<rangle> [\<Down>]\<^sub>t Val (VRef r); 
+       Pr, \<Delta>, get_valid_locs \<omega>0 \<turnstile> \<langle>e_p; \<omega>\<rangle> [\<Down>]\<^sub>t Val (VPerm p);
        a = the_address r \<rbrakk> \<Longrightarrow>
        red_exhale Pr \<Delta> \<omega>0 (Atomic (Acc e_r f (PureExp e_p))) (m,pm) 
                            (exh_if_total (p \<ge> 0 \<and> pgte (m(a,f)) (Abs_prat p) \<and> r \<noteq> Null) (m( (a,f) := psub (m (a,f)) (Abs_prat p)),pm)) "
 
  \<comment>\<open>Exhaling wildcard removes some non-zero permission that this is less than the current permission held\<close>
   | ExhAccWildcard:
-    "\<lbrakk> \<omega> = update_mask_total_full \<omega>0 m;
-       Pr, \<Delta>, Some (get_valid_locs \<omega>0) \<turnstile> \<langle>e_r; \<omega>\<rangle> [\<Down>]\<^sub>t Val (VRef r);
+    "\<lbrakk> \<omega> = update_mh_total_full \<omega>0 m;
+       Pr, \<Delta>, get_valid_locs \<omega>0 \<turnstile> \<langle>e_r; \<omega>\<rangle> [\<Down>]\<^sub>t Val (VRef r);
        q \<in> {p. p \<noteq> pnone \<and> pgt (m(a,f)) q} \<rbrakk> \<Longrightarrow>
        red_exhale Pr \<Delta> \<omega>0 (Atomic (Acc e_r f Wildcard)) (m,pm) 
                            (exh_if_total (m(a,f) \<noteq> pnone \<and> r \<noteq> Null) 
@@ -54,15 +54,15 @@ inductive red_exhale :: "program \<Rightarrow> 'a interp \<Rightarrow> 'a full_t
 
 \<comment>\<open>exhale acc(P(es), p)\<close>
   | ExhAccPred:
-     "\<lbrakk> \<omega> = update_mask_total_full \<omega>0 m;
-       red_pure_exps_total Pr \<Delta> (Some (get_valid_locs \<omega>)) e_args \<omega> (map Val v_args);
-       Pr, \<Delta>, Some (get_valid_locs \<omega>0) \<turnstile> \<langle>e_p; \<omega>\<rangle> [\<Down>]\<^sub>t Val (VPerm p) \<rbrakk> \<Longrightarrow>
+     "\<lbrakk> \<omega> = update_mh_total_full \<omega>0 m;
+       red_pure_exps_total Pr \<Delta> (get_valid_locs \<omega>) e_args \<omega> (map Val v_args);
+       Pr, \<Delta>, get_valid_locs \<omega>0 \<turnstile> \<langle>e_p; \<omega>\<rangle> [\<Down>]\<^sub>t Val (VPerm p) \<rbrakk> \<Longrightarrow>
       red_exhale Pr \<Delta> \<omega>0 (Atomic (AccPredicate pred_id e_args (PureExp e_p))) (m,pm)
               (exh_if_total (p \<ge> 0 \<and> pgte (pm(pred_id, v_args)) (Abs_prat p) \<and> r \<noteq> Null) 
                             (m, pm( (pred_id, v_args) := psub (pm (pred_id, v_args)) (Abs_prat p))))"
   | ExhAccPredWildcard:
-    "\<lbrakk> \<omega> = update_mask_total_full \<omega>0 m;
-       red_pure_exps_total Pr \<Delta> (Some (get_valid_locs \<omega>)) e_args \<omega> (map Val v_args);
+    "\<lbrakk> \<omega> = update_mh_total_full \<omega>0 m;
+       red_pure_exps_total Pr \<Delta> (get_valid_locs \<omega>) e_args \<omega> (map Val v_args);
        q \<in> {p. p \<noteq> pnone \<and> pgt (m(a,f)) q} \<rbrakk> \<Longrightarrow>
        red_exhale Pr \<Delta> \<omega>0 (Atomic (AccPredicate pred_id e_args Wildcard)) (m,pm) 
                            (exh_if_total (m(a,f) \<noteq> pnone)
@@ -70,12 +70,12 @@ inductive red_exhale :: "program \<Rightarrow> 'a interp \<Rightarrow> 'a full_t
 
 \<comment>\<open>exhale other cases\<close>
   | ExhPure:
-    "\<lbrakk> \<omega> = update_mask_total_full \<omega>0 m; 
-       Pr, \<Delta>, Some (get_valid_locs \<omega>0) \<turnstile> \<langle>e; \<omega>\<rangle> [\<Down>]\<^sub>t Val (VBool b) \<rbrakk> \<Longrightarrow>
+    "\<lbrakk> \<omega> = update_mh_total_full \<omega>0 m; 
+       Pr, \<Delta>, get_valid_locs \<omega>0 \<turnstile> \<langle>e; \<omega>\<rangle> [\<Down>]\<^sub>t Val (VBool b) \<rbrakk> \<Longrightarrow>
        red_exhale Pr \<Delta> \<omega>0 (Atomic (Pure e)) (m,pm) (if b then ExhaleNormal (m,pm) else ExhaleFailure)"
   | SubAtomicFailure: 
     "\<lbrakk> e \<in> sub_expressions_atomic A ;
-      Pr, \<Delta>, Some (get_valid_locs \<omega>0) \<turnstile> \<langle>e; \<omega>\<rangle> [\<Down>]\<^sub>t VFailure  \<rbrakk> \<Longrightarrow> 
+      Pr, \<Delta>, get_valid_locs \<omega>0 \<turnstile> \<langle>e; \<omega>\<rangle> [\<Down>]\<^sub>t VFailure  \<rbrakk> \<Longrightarrow> 
        red_exhale Pr \<Delta> \<omega>0 (Atomic A) (m,pm) ExhaleFailure"
 
 \<comment>\<open>exhale A && B\<close>
@@ -89,35 +89,41 @@ inductive red_exhale :: "program \<Rightarrow> 'a interp \<Rightarrow> 'a full_t
 
 \<comment>\<open>exhale A \<longrightarrow> B\<close>
  | ExhImpTrue: 
-   "\<lbrakk>  \<omega> = update_mask_and_pmask_total_full \<omega>0 (fst m_pm) (snd m_pm);
-      Pr, \<Delta>, Some (get_valid_locs \<omega>0) \<turnstile> \<langle>e; \<omega>\<rangle> [\<Down>]\<^sub>t Val (VBool True); 
+   "\<lbrakk>  \<omega> = update_m_total_full \<omega>0 (fst m_pm) (snd m_pm);
+      Pr, \<Delta>, get_valid_locs \<omega>0 \<turnstile> \<langle>e; \<omega>\<rangle> [\<Down>]\<^sub>t Val (VBool True); 
       red_exhale Pr \<Delta> \<omega>0 A m_pm res \<rbrakk> \<Longrightarrow>
       red_exhale Pr \<Delta> \<omega>0 (Imp e A) m_pm res" 
  | ExhImpFalse:  
-   "\<lbrakk> \<omega> = update_mask_and_pmask_total_full \<omega>0 (fst m_pm) (snd m_pm);
-      Pr, \<Delta>, Some (get_valid_locs \<omega>0) \<turnstile> \<langle>e; \<omega>\<rangle> [\<Down>]\<^sub>t Val (VBool False) \<rbrakk> \<Longrightarrow> 
+   "\<lbrakk> \<omega> = update_m_total_full \<omega>0 (fst m_pm) (snd m_pm);
+      Pr, \<Delta>, get_valid_locs \<omega>0 \<turnstile> \<langle>e; \<omega>\<rangle> [\<Down>]\<^sub>t Val (VBool False) \<rbrakk> \<Longrightarrow> 
       red_exhale Pr \<Delta> \<omega>0 (Imp e A) m_pm (ExhaleNormal m_pm)"
  | ExhImpFailure:
-   "\<lbrakk> \<omega> = update_mask_and_pmask_total_full \<omega>0 (fst m_pm) (snd m_pm); 
-      Pr, \<Delta>, Some (get_valid_locs \<omega>0) \<turnstile> \<langle>e; \<omega>\<rangle> [\<Down>]\<^sub>t VFailure \<rbrakk> \<Longrightarrow> 
+   "\<lbrakk> \<omega> = update_m_total_full \<omega>0 (fst m_pm) (snd m_pm); 
+      Pr, \<Delta>, get_valid_locs \<omega>0 \<turnstile> \<langle>e; \<omega>\<rangle> [\<Down>]\<^sub>t VFailure \<rbrakk> \<Longrightarrow> 
      red_exhale Pr \<Delta> \<omega>0 (Imp e A) m_pm ExhaleFailure"
 
-record conf =
-  havoc_inhale :: bool
 
+definition havoc_undef_locs :: "'a total_heap \<Rightarrow> 'a predicate_heap \<Rightarrow> mask \<Rightarrow> 'a predicate_mask \<Rightarrow> ('a total_heap \<times> 'a predicate_heap) set"
+  where "havoc_undef_locs hh hp mh mp = 
+           { (hh', hp') | hh' hp'. 
+                (\<forall>lh. mh lh \<noteq> pnone \<longrightarrow> hh' lh = hh lh) \<and>
+                (\<forall>lp. mp lp \<noteq> pnone \<longrightarrow> 
+                          hp' lp = hp lp \<and>
+                         (\<forall>lh \<in> get_lhset_pheap hp lp. hh' lh = hh lh) \<and>
+                         (\<forall>lp2 \<in> get_lpset_pheap hp lp. hp' lp2 = hp lp2)) }"
 
-(* alternative:
-definition havoc_undef_locs :: "'a full_total_state \<Rightarrow> mask \<Rightarrow> 'a full_total_state set"
-  where "havoc_undef_locs \<omega> m = {\<omega>'| \<omega>'. \<forall>l. pgt (m l) pnone \<longrightarrow> get_heap_total_full \<omega> l = get_heap_total_full \<omega>' l}"
-*)
-definition havoc_undef_locs :: "'a total_heap \<Rightarrow> 'a predicate_heap \<Rightarrow> mask \<Rightarrow> 'a predicate_mask \<Rightarrow> 'a total_heap set"
-  where "havoc_undef_locs h m pm = {h' | h'. \<forall>l. pgt (m l) pnone \<longrightarrow> h' l = h l}"
+text\<open>\<^term>\<open>havoc_undef_locs hh hp mh mp\<close> denotes the set of heaps that coincide with \<^term>\<open>(hh,hp)\<close> w.r.t.
+the permission masks \<^term>\<open>(mh,mp)\<close>. This means the heaps agree on all heap and predicate locations for 
+which direct permission is held in \<^term>\<open>(mh,mp)\<close> or which is part of a predicate snapshot in \<^term>\<open>hp\<close> 
+of a directly owned (w.r.t. \<^term>\<open>mp\<close>) predicate\<close>
 
-definition exhale_state :: "'a full_total_state \<Rightarrow> mask \<Rightarrow> 'a full_total_state set"
-  where "exhale_state \<omega> m = {\<omega>' | \<omega>'. get_store_total \<omega>' = get_store_total \<omega> \<and>
-                                      get_trace_total \<omega>' = get_trace_total \<omega> \<and>
-                                      get_mask_total_full \<omega>' = m \<and>
-                                      get_heap_total_full \<omega>' \<in> havoc_undef_locs (get_heap_total_full \<omega>) m}"
+definition exhale_state :: "'a full_total_state \<Rightarrow> mask \<times> 'a predicate_mask \<Rightarrow> 'a full_total_state set"
+  where "exhale_state \<omega> m = 
+    {\<omega>' | \<omega>'. get_store_total \<omega>' = get_store_total \<omega> \<and>
+              get_trace_total \<omega>' = get_trace_total \<omega> \<and>
+              get_m_total_full \<omega>' = m \<and>
+              get_h_total_full \<omega>' \<in> 
+                   havoc_undef_locs (get_hh_total_full \<omega>) (get_hp_total_full \<omega>) (fst m) (snd m)}"
 
 lemma exhale_state_same_store: "\<omega>' \<in> exhale_state \<omega> m \<Longrightarrow> get_store_total \<omega>' = get_store_total \<omega>"
   by (simp add: exhale_state_def)
@@ -125,76 +131,74 @@ lemma exhale_state_same_store: "\<omega>' \<in> exhale_state \<omega> m \<Longri
 lemma exhale_state_same_trace: "\<omega>' \<in> exhale_state \<omega> m \<Longrightarrow> get_trace_total \<omega>' = get_trace_total \<omega>"
   by (simp add: exhale_state_def)
 
-fun map_option_2 :: "('a \<Rightarrow> 'b) \<Rightarrow> 'b \<Rightarrow> 'a option \<Rightarrow> 'b"
-  where 
-    "map_option_2 f y None = y"
-  | "map_option_2 f _ (Some x) = f x"
-      
-
 (* Currently, red_stmt_total_single is a function. But if angelism is added, then it would not be a 
 function *) (* inhale (acc(x.f) && x.f = 5 \<Longrightarrow> 0/0 = 0/0) *)
-inductive red_stmt_total_single_set :: "program \<Rightarrow> 'a interp \<Rightarrow> conf \<Rightarrow> stmt \<Rightarrow> 'a full_total_state  \<Rightarrow> (stmt+unit) \<times> ('a standard_result) \<Rightarrow> bool"
-  for Pr :: program and \<Delta> :: "'a interp" and conf :: conf where
-   RedSkip: " red_stmt_total_single_set Pr \<Delta> conf Skip \<omega> (Inr (), RNormal \<omega>)" 
+
+inductive red_stmt_total_single_set :: "program \<Rightarrow> 'a interp \<Rightarrow> stmt \<Rightarrow> 'a full_total_state  \<Rightarrow> (stmt+unit) \<times> ('a standard_result) \<Rightarrow> bool"
+  for Pr :: program and \<Delta> :: "'a interp" where
+   RedSkip: " red_stmt_total_single_set Pr \<Delta> Skip \<omega> (Inr (), RNormal \<omega>)" 
  | RedInhale: 
-   "\<lbrakk> red_inhale Pr \<Delta> (havoc_inhale conf) A \<omega> res \<rbrakk> \<Longrightarrow>
-      red_stmt_total_single_set Pr \<Delta> conf (Inhale A) \<omega> (Inr (), res)"
+   "\<lbrakk> red_inhale Pr \<Delta> A \<omega> res \<rbrakk> \<Longrightarrow>
+      red_stmt_total_single_set Pr \<Delta> (Inhale A) \<omega> (Inr (), res)"
  | RedExhale: 
    "\<lbrakk> red_exhale Pr \<Delta> \<omega> A (get_mask_total_full \<omega>) (ExhaleNormal m');
       \<omega>' \<in> exhale_state \<omega> m' \<rbrakk> \<Longrightarrow>
-      red_stmt_total_single_set Pr \<Delta> conf (Exhale A) \<omega> (Inr (), RNormal \<omega>')"
+      red_stmt_total_single_set Pr \<Delta> (Exhale A) \<omega> (Inr (), RNormal \<omega>')"
  | RedExhaleFailure:
    "\<lbrakk> red_exhale Pr \<Delta> \<omega> A (get_mask_total_full \<omega>) ExhaleFailure \<rbrakk> \<Longrightarrow>
-      red_stmt_total_single_set Pr \<Delta> conf (Exhale A) \<omega> (Inr (), RFailure)"
+      red_stmt_total_single_set Pr \<Delta> (Exhale A) \<omega> (Inr (), RFailure)"
  | RedAssert:
    "\<lbrakk> red_exhale Pr \<Delta> \<omega> A (get_mask_total_full \<omega>) (ExhaleNormal m') \<rbrakk> \<Longrightarrow>
-      red_stmt_total_single_set Pr \<Delta> conf (Assert A) \<omega> (Inr (), RNormal \<omega>)"
+      red_stmt_total_single_set Pr \<Delta> (Assert A) \<omega> (Inr (), RNormal \<omega>)"
  | RedAssertFailure:
    "\<lbrakk> red_exhale Pr \<Delta> \<omega> A (get_mask_total_full \<omega>) ExhaleFailure \<rbrakk> \<Longrightarrow>
-      red_stmt_total_single_set Pr \<Delta> conf (Assert A) \<omega> (Inr (), RFailure)"
+      red_stmt_total_single_set Pr \<Delta> (Assert A) \<omega> (Inr (), RFailure)"
+
+
 \<comment>\<open>TODO: Add semantics for \<^term>\<open>Assume A\<close>. Should be the same as \<^term>\<open>Assert A\<close>, except that 
         \<^term>\<open>Assert A\<close> goes to failure iff \<^term>\<open>Assume A\<close> goes to magic. The back-ends implement it
         differently correctly. \<close>
- (*| RedAssume: "red_stmt_total_single_set Pr conf (Assume A) \<omega> (Inr (), (handle_inhale Pr (havoc_inhale conf) True A \<omega>))"*)
-(* | RedExhale: "red_stmt_total_single_set Pr conf (Exhale A) \<omega> 
+ (*| RedAssume: "red_stmt_total_single_set Pr (Assume A) \<omega> (Inr (), (handle_inhale Pr (havoc_inhale conf) True A \<omega>))"*)
+(* | RedExhale: "red_stmt_total_single_set Pr (Exhale A) \<omega> 
                      (Inr (), map_option_2 (\<lambda>xs. Set (\<Union>m \<in> xs. exhale_state \<omega> m)) Failure (handle_exhale_2 Pr \<omega> A (get_total_mask_full \<omega>)))"*)
  | RedLocalAssign:
-   "\<lbrakk> wd_pure_exp_total Pr \<Delta> CInhale e \<omega>; Pr, \<Delta> \<turnstile> \<langle>e; \<omega>\<rangle> [\<Down>]\<^sub>t (Val v) \<rbrakk> \<Longrightarrow> 
-     red_stmt_total_single_set Pr \<Delta> conf (LocalAssign x e) \<omega> (Inr (), (RNormal (update_store_total \<omega> x v)))"
- | RedLocalAssignFailure: 
+   "\<lbrakk> Pr, \<Delta>, Some (get_valid_locs \<omega>) \<turnstile> \<langle>e; \<omega>\<rangle> [\<Down>]\<^sub>t (Val v) \<rbrakk> \<Longrightarrow> 
+     red_stmt_total_single_set Pr \<Delta> (LocalAssign x e) \<omega> (Inr (), (RNormal (update_store_total \<omega> x v)))"
+(*
+| RedLocalAssignFailure:
    "\<lbrakk> \<not> wd_pure_exp_total Pr \<Delta> CInhale e \<omega> \<rbrakk> \<Longrightarrow> 
-   red_stmt_total_single_set Pr \<Delta> conf (LocalAssign x e) \<omega> (Inr (), RFailure)"
+   red_stmt_total_single_set Pr \<Delta> (LocalAssign x e) \<omega> (Inr (), RFailure)"
  | RedFieldAssign: 
    "\<lbrakk> wd_pure_exp_total Pr \<Delta> CInhale e_r \<omega>; 
       wd_pure_exp_total Pr \<Delta> CInhale e \<omega>; 
       Pr, \<Delta> \<turnstile> \<langle>e_r; \<omega>\<rangle> [\<Down>]\<^sub>t Val (VRef (Address addr));
       get_mask_total_full \<omega> (addr,f) \<noteq> pnone;
       Pr, \<Delta>  \<turnstile> \<langle>e; \<omega>\<rangle> [\<Down>]\<^sub>t Val v \<rbrakk> \<Longrightarrow> 
-      red_stmt_total_single_set Pr \<Delta> conf (FieldAssign e_r f e) \<omega> (Inr (), (RNormal (update_heap_total_full \<omega> (addr,f) v)))"
+      red_stmt_total_single_set Pr \<Delta> (FieldAssign e_r f e) \<omega> (Inr (), (RNormal (update_heap_total_full \<omega> (addr,f) v)))"
  | RedFieldAssignFailure: 
    "\<lbrakk> \<not> wd_pure_exp_total Pr \<Delta> CInhale e_r \<omega> \<or> 
       \<not> wd_pure_exp_total Pr \<Delta> CInhale e \<omega> \<or> 
       (Pr, \<Delta> \<turnstile> \<langle>e_r; \<omega>\<rangle> [\<Down>]\<^sub>t Val (VRef Null)) \<or> 
       get_mask_total_full \<omega> (addr,f) \<noteq> pnone \<rbrakk> \<Longrightarrow> 
-      red_stmt_total_single_set Pr \<Delta> conf (FieldAssign e_r f e) \<omega> (Inr (), RFailure)"
+      red_stmt_total_single_set Pr \<Delta> (FieldAssign e_r f e) \<omega> (Inr (), RFailure)"
  | RedIfTrue: 
    "\<lbrakk> Pr,\<Delta> \<turnstile> \<langle>e_b; \<omega>\<rangle> [\<Down>]\<^sub>t Val (VBool True);
      wd_pure_exp_total Pr \<Delta> CInhale e_b \<omega> \<rbrakk> \<Longrightarrow> 
-      red_stmt_total_single_set Pr \<Delta> conf (If e_b s1 s2) \<omega> (Inl s1, RNormal \<omega>)"
+      red_stmt_total_single_set Pr \<Delta> (If e_b s1 s2) \<omega> (Inl s1, RNormal \<omega>)"
  | RedIfFalse: 
    "\<lbrakk> Pr,\<Delta> \<turnstile> \<langle>e_b; \<omega>\<rangle> [\<Down>]\<^sub>t Val (VBool False);
       wd_pure_exp_total Pr \<Delta> CInhale e_b \<omega> \<rbrakk> \<Longrightarrow> 
-      red_stmt_total_single_set Pr \<Delta> conf (If e_b s1 s2) \<omega> (Inl s2, RNormal \<omega>)"
+      red_stmt_total_single_set Pr \<Delta> (If e_b s1 s2) \<omega> (Inl s2, RNormal \<omega>)"
  | RedIfFailure:
     "\<lbrakk> \<not>wd_pure_exp_total Pr \<Delta> CInhale e_b \<omega> \<rbrakk> \<Longrightarrow>
-       red_stmt_total_single_set Pr \<Delta> conf (If e_b s1 s2) \<omega> (Inr (), RFailure)"
+       red_stmt_total_single_set Pr \<Delta> (If e_b s1 s2) \<omega> (Inr (), RFailure)"
  | RedSeq1:
-   "\<lbrakk> red_stmt_total_single_set Pr \<Delta> conf s1 \<omega> (Inl s'', r'') \<rbrakk> \<Longrightarrow>
-      red_stmt_total_single_set Pr \<Delta> conf (Seq s1 s2) \<omega> (Inl (Seq s'' s2), r'')"
+   "\<lbrakk> red_stmt_total_single_set Pr \<Delta> s1 \<omega> (Inl s'', r'') \<rbrakk> \<Longrightarrow>
+      red_stmt_total_single_set Pr \<Delta> (Seq s1 s2) \<omega> (Inl (Seq s'' s2), r'')"
  | RedSeq2: 
-   "\<lbrakk> red_stmt_total_single_set Pr \<Delta> conf s1 \<omega> (Inr (), r'') \<rbrakk> \<Longrightarrow>
-      red_stmt_total_single_set Pr \<Delta> conf (Seq s1 s2) \<omega> (Inl s2, r'')"
-
+   "\<lbrakk> red_stmt_total_single_set Pr \<Delta> s1 \<omega> (Inr (), r'') \<rbrakk> \<Longrightarrow>
+      red_stmt_total_single_set Pr \<Delta> (Seq s1 s2) \<omega> (Inl s2, r'')"
+*)
 type_synonym 'a stmt_config = "(stmt + unit) \<times> 'a standard_result"
 
 inductive red_stmt_total_single :: "program \<Rightarrow> 'a interp \<Rightarrow> conf \<Rightarrow> 'a stmt_config \<Rightarrow> 'a stmt_config \<Rightarrow> bool"
